---
title: "12.2"
date: 2025-01-31 14:28:33
feed: show
---
### 3.1

#### 2
$$
\begin{flalign}
&\text{(1)}\int 3x^4 dx = \dfrac{3}{5} x^5 +C \\
&\text{(2)} \int \sqrt{x\sqrt x} \, dx=\int x^{\dfrac{3}{4}}dx =\dfrac{4}{7} x^{\dfrac{7}{4}} + C \\
& \text{(3)} \int \dfrac{1}{x \cdot \sqrt[3]{x}} dx = \int x^{-\dfrac{3}{4}}dx = 4x^{\dfrac{1}{4}} + C\\
&\text{(4)} \int (1-2x)^2dx = - \dfrac{(1-2x)^3}{6} + C\\
&(5)\int \dfrac{(1-x)^2}{x}dx = \int(x-2+\dfrac{1}{x})dx = \dfrac{1}{2}x^2 -2x +\ln x + C \\
&(6)\int \dfrac{2x^4+3x^2+4}{x^2+1}dx = \int(2x^2+1+\dfrac{3}{x^2+1})dx =\dfrac{2}{3}x^3+x+3\arctan x +C \\
&(8) \int \dfrac{(1-x)^2}{\sqrt{x}} dx  = \int (x^{\dfrac{3}{2}} - 2 x^{\dfrac{1}{2}} + x^{-\dfrac{1}{2}})dx = \dots  \\
&(9) \int e^x (1 - \dfrac{e^{-x}}{x})dx = \int (e^x - \dfrac{1}{x})dx = e^x - \ln x + C \\
&(11) \int \dfrac{5 \cdot 2^x + 2 \cdot 5^x}{5^x}dx = \int(5 \cdot (\dfrac{2}{5})^x + 2)dx = 2x + \dfrac{5}{\ln \dfrac{2}{5}} \cdot (\dfrac{2}{5})^x + C \\
&(12) \int \cos ^2 \dfrac{x}{2}dx = \int (1-\sin ^2 \dfrac{x}{2})dx = x - 4\sin ^2 \dfrac{x}{4} +C \\
&(14) \int \dfrac{2}{1-\cos 2x} dx = \int \csc ^ 2 x \; dx = -\cot x + C \\
&(15) \int \dfrac{1+ \sin x}{1 + \cos 2x} dx = \int \dfrac{1+ \sin x}{2 \cos ^2 x}dx = \dfrac{1+ \sin x}{\cos x} + C \\
&(16) \int \dfrac{1}{1 + \sin x}dx = \int \dfrac{1 - \sin x}{\cos ^2 x}dx = \dfrac{\sin x - 1}{\cos x} + C \\
&(17) \int \dfrac{1+x+x^2}{x(1+x^2)}dx = \int \dfrac{1}{x} dx + \int \dfrac{x}{1+x^2}dx = \ln |x| + \dfrac{\ln (1+x^2)}{2}+C \\
&(18) \int \dfrac{1}{x^2 (1+x^2)}=\int \dfrac{1}{x^2}dx - \int \dfrac{1}{1+x^2}dx = -\dfrac{1}{x} -\arctan x +C \\
\end{flalign}
$$

#### 3
$$
\begin{flalign}
\int f(x)dx = \begin{cases}
\dfrac{1}{2}x^2 +2x+C & \quad x \geq0 \\
-\dfrac{1}{2}x^2 +2x+C & \quad x < 0
\end{cases}
\end{flalign}
$$

---
### 3.2
#### 2
(2)
$$
\begin{flalign}
\int e^{4x-5} dx = \dfrac{1}{4} e^{4x-5}+C \\
\end{flalign}
$$

(4)
令$u = 1-2x^2$ ，则$du= -4x \, dx$ 

$$
\begin{flalign}
\int x(1-2x^2)^3dx &=  \int u^3 \cdot (-\dfrac{1}{4})du \\
&=-\dfrac{1}{16}u^4 +C\\
&=-\dfrac{1}{16}(1-2x^2)^4+C
\end{flalign}
$$

(5)
$$
\begin{flalign}
\int \dfrac{1}{4-9x^2} dx &= \int \dfrac{1}{4(2+3x)} dx +\int \dfrac{1}{4(2-3x)}dx \\
& = \dfrac{ln(2+3x)}{12} - \dfrac{ln(2-3x)}{12} +C \\
\end{flalign}
$$

(6)
$$
\begin{align}
\int \dfrac{\cos {\sqrt{x}}}{\sqrt{x}}dx = 2\sin{\sqrt{x}} +C
\end{align}
$$

(7)
令 $u=\sqrt{1+x^2}$ 
$$
\begin{align}
\int \sec{\sqrt{1+x^2}} \cdot \dfrac{x}{\sqrt{1+x^2}}dx &= \int \sec {u} \cdot du \\
&=\int \dfrac{\sec{u}(\sec{u} + \tan{u})}{\sec{u}+\tan{u}}du
\end{align}
$$
令$\mu = \sec{u}+\tan{u}$ 
$$
\begin{align}
\text{原式}=&\int \dfrac{d \mu}{\mu} \\
=& \ln |\mu| +C \\
=& \ln|\sec{u} + \tan{u} | +C \\
=& \ln|\sec{\sqrt{1+x^2}} + \tan{\sqrt{1+x^2}}| +C \\
\end{align}
$$

(9)
$$
\begin{align}
\int \dfrac{x}{\sqrt{3-4x^2}}dx = -\dfrac{1}{4}\sqrt{3-4x^2} +C \\
\end{align}
$$

(11)
令 $u=sinx$ 
$$
\begin{align}
\int \dfrac{\sin{x} \cos{x}}{1+\sin ^4 x}dx =&\int \dfrac{u}{1+u^4}du \\
=& \dfrac{1}{2} \int \dfrac{2u}{1+u^4} du \\
=& \dfrac{1}{2} \int \dfrac{1}{1+(u^2)^2}du^2 \\
=& \dfrac{1}{2} \arctan u^2 +C \\
=& \dfrac{1}{2} \arctan \sin^2x +C \\
\end{align}
$$


(14)
$$
\begin{align}
\int \cos ^4 xdx =& \int \dfrac{1}{4}(\cos^22x + 2\cos 2x +1)dx \\
=& \dfrac{1}{4}\int \cos^22x \, dx \; + \dfrac{1}{4}\sin 2x + \dfrac{1}{4}x+C \\
=& \dfrac{1}{4} \int \dfrac{\cos 4x + 1}{2}dx + \dfrac{1}{4}sin2x +\dfrac{1}{4}x+C \\
=& \dots
\end{align}
$$

(15)
令$u= \cos x$ 
$$
\begin{align}
\int sin^3 x\, cos^2xdx =& \int (1-\cos ^2 x)\cos^2x \cdot \sin x dx \\
=&\int(u^2-1)u^2 du \\
=& \dfrac{1}{5}u^5-\dfrac{1}{3}u^3+C \\
=& \dfrac{1}{5} \cos^5x - \dfrac{1}{3} \cos^5x +C \\
\end{align}
$$

(18)
$$
\begin{align}
\int \sec ^4x dx =& \int (\tan^2 x+1)d\tan x \\
=& \dfrac{1}{3}\tan^3x + \tan x +C \\
\end{align}
$$

(19)
$$
\begin{align}
\int \sec ^3 x \cdot \tan x dx =& \int (\sec x)^2 d\sec x \\
=& \dfrac{1}{3}\sec^3 x +C \\
\end{align}
$$

---

### 3.3
#### 1
$$
\begin{aligned}
(1) &\int \ln x dx = x \ln x -x +C 
\end{aligned}
$$
$$
\begin{aligned}
(2) &\int \arcsin xdx = x \arcsin x + \sqrt{1-x^2} +C \\
\end{aligned}
$$
$$
\begin{aligned}
(4) \int (x^2 +2x +5)e^{-3x}dx =& -\dfrac{1}{3}\int (x^2+2x+5)de^{-3x} \\
=& -\dfrac{1}{3}
\end{aligned}
$$



