---
title: "3.6"
date: 2025-01-31 14:28:34
feed: show
---
### 1
+ (3)
$$
\begin{align}
\text{设} \; \mathrm{F}'(t) =e^{t^2} \\ 
 \dfrac{\mathrm{d}}{\mathrm{d}x}(\mathrm{F}(\sin x)-\mathrm{F}(a))&= \mathrm{F}'(\sin x) \cdot \cos x \\
 & =e^{(\sin x)^2} \cdot \cos x \\
\end{align}
$$
+ (4) 
$$
\begin{align}
\text{设} \mathrm{F}'(t) = \cos(t^2) \\
\dfrac{\mathrm{d}}{\mathrm{d}x}y = & \dfrac{\mathrm{d}}{\mathrm{d}x} (\mathrm{F}(\ln x)-\mathrm{F}(x^2)) \\
=&\dfrac{\mathrm{F}'(\ln x)}{x} - 2x\mathrm{F}'(x^2) \\
=&\dfrac{\cos((\ln x)^2)}{x} - 2x\cos (x^4)\\
\end{align}
$$
+ (5)
$$
\begin{aligned}
\dfrac{\mathrm{d}y}{\mathrm{d}x} \ln y - \dfrac{\mathrm{d} (xy)}{\mathrm{d}x} \cdot\arctan (xy) = 0 \\
\dfrac{\mathrm{d}y}{\mathrm{d}x} \ln y - y - x \cdot \arctan (xy) \dfrac{\mathrm{d}y}{\mathrm{d}x} = 0 \\
\dfrac{\mathrm{d}y}{\mathrm{d}x} = \dfrac{y}{\ln y - x \arctan(xy)} \\
\end{aligned}
$$
+ (6)
$$
\begin{align}
\dfrac{\mathrm{d}y}{\mathrm{d}x} = \dfrac{\dfrac{\mathrm{d}y}{\mathrm{d}t}}{\dfrac{\mathrm{d}x}{\mathrm{d}t}} = \dfrac{\sin(t^2)}{-2t \dfrac{\sin (t^2)}{t^2}} = -\dfrac{t}{2} \\
\end{align}
$$
### 2
+ (3) 
$$
\begin{align}
\int_{\dfrac{\pi}{4}}^{\dfrac{\pi}{2}} \dfrac{1+\sin ^2 x}{1 - \cos 2x} \mathrm{d}x&=\int_{\dfrac{\pi}{4}}^{\dfrac{\pi}{2}} \dfrac{1+\sin ^2}{2\sin ^2x} \mathrm{d}x \\
& = \dfrac{1}{2}\int_{\dfrac{\pi}{4}}^{\dfrac{\pi}{2}} (\dfrac{1}{\sin^2x} + 1) \mathrm{d} x \\
&=\dfrac{1}{2} ()

\end{align}
$$
+ (5)
$$
\begin{align}
\int_0^3 \sqrt{x^2 -2x +1} \mathrm{d}x = & \int_0^3 |x-1| \mathrm{d}x =\int_0^1(1-x)\mathrm{d}x + \int_1^3 (x-1)\mathrm{d}x = 2
\end{align}
$$
+ (6)
$$
\begin{align}
\int_{-2}^3 f(x) \mathrm{d}x = \int_{-2}^0 (2+x) \mathrm{d}x + \int_0^3 (1-x^2) \mathrm{d}x = -4 \\
\end{align}
$$
### 3
+ (2)
$$
\begin{align}
&\text{由洛必达定理得：} \\
&\lim_{x \to 0}\dfrac{\int_0^{x^2} \dfrac{\tan t}{t} \mathrm{d}t}{\int_0^x \arcsin t \mathrm{d}t}= \lim_{x \to 0} \dfrac{\dfrac{\tan x^2}{x^2}\cdot (2x)}{\arcsin x} =2 
\end{align}
$$
+ (4) 
$$
\begin{align}
\text{原极限} = \lim_{x \to 0} \dfrac{xf(x)}{xf(0)} = 1 \\ 
\end{align}
$$
### 4
$$
\begin{align}
&\text{当}x \leq 0 \text{时：}  \\
&\Phi(x) = \int_{-1}^x e^{-t} \mathrm{d}t = -e^{-x}+e \\
&\text{当} x > 0 \text{时：} \\
&\Phi(x) = -1+e + \int_0^xt \mathrm{d}t =\dfrac{1}{2} x^2+e-1 \\ 
\end{align}
$$
