$$
\begin{align}
&=\int x\,df(x) = xf(x)-\int f(x)dx \\
&= x \cdot (\cos x \,\ln x + \dfrac{1+\sin x}{x}) -(1+\sin x)\ln x +C \\
\\
&1^o \quad \int \dfrac{dx}{1+\sqrt{1-x^2}} \\
&\text{Let} \; x = \sin t \quad t\in (-\dfrac{\pi}{2},\dfrac{\pi}{2}) \\
&\text{原式}=\int \dfrac{1}{1+\cos t}d\sin t = \int \dfrac{\cos t}{1+\cos t}dt \\
\\
&\dfrac{\sqrt{x^2+1}}{x} = \sqrt{\dfrac{x^2+1}{x^2}} \\
\\
 V &= \int_0^{2\pi a} \pi (y-2a)^2 \mathrm{d} x \\
&= \int_0^{2 \pi a} \pi a^2(1+\cos t)^2 \mathrm{d} [a(t - \sin t)] \\
&= \int_0^{2 \pi} \pi a^2(1+\cos t)^2 \cdot a(1-\cos t) \mathrm{d}t \\
& = \pi a^3 \int ... \\
\int_0^{2\pi} (1+\cos t)^2 (1-\cos t) \mathrm{d}t &= \int_0^{2\pi} (1+\cos t)\sin^2t \mathrm{d} t \\
&=\int_0^{2\pi} \sin^2 t \mathrm{d}t + \int_0^{2\pi} \sin^2 t \mathrm{d} \sin t \\
&= \int_0^{2\pi} \dfrac{1-\cos 2t}{2} \mathrm{d}t + \int_0^{2\pi} \sin^2 t \mathrm{d} \sin t \\
&= \\
\\

\end{align}
$$
$$
\begin{align}
V_{\text{间隙}} &= \int_0^2 \pi \cdot (2x - x^2 -1)^2 \; \mathrm{d}x  \\
&= \pi \cdot \int_0^2 (x-1)^4  \; \mathrm{d}(x-1) \\
&= \pi \cdot \dfrac{1}{5}(x-1)^5 |_0^2 \\
&= \dfrac{2 \pi}{5} \\
V_{\text{所求}} &= V_{\text{圆柱}} - V_{\text{间隙}} \\
&= \pi \cdot 1 \cdot 2 - \dfrac{2 \pi}{5} \\
&= \dfrac{8}{5} \pi \\
\\
\\
Y =& y - 1 = 2x -x^2 -1 = -(x-1)^2 \\
\\
V &= \int_{-1}^0 (x-1)^2 \pi \; \mathrm{d}Y \\
&= \pi \int_{-1}^0 -Y \;\mathrm{d}Y \\
&=\pi \cdot -\frac{1}{2}Y^2|_{-1}^0 \\
& = \frac{\pi}{2} \\

\\
\\
\end{align}
$$
### 计算题
#### 1.
   a、
$$
\begin{align}
\cos \theta = \frac{\boldsymbol{A} \cdot \boldsymbol{B}}{|\boldsymbol{A}| \cdot |\boldsymbol{B}|} =\frac{11}{\sqrt{13} \times \sqrt{17}} = \frac{11}{\sqrt{211}}
\end{align}
$$
   b、
$$
\begin{align}
S=|\boldsymbol{A} \times \boldsymbol{B}| = |(2 \times 1) - (3 \times 4) |= 10
\end{align}
$$
#### 2.
$\boldsymbol{A} \cdot \boldsymbol{B} = 0$ ，所以 **A** 和 **B** 垂直
#### 3.
$$
\begin{align}
\int x \ln x\; dx = \int \frac{1}{2} \cdot 2 \cdot x \ln x \;dx = \frac{1}{2} \int \ln x \; \cdot 2xdx = \frac{1}{2}\int \ln x  \; dx^2
\end{align}
$$

---
1. **直接代入法就相当于`v=v(t), u=u(t)`**
$$
\begin{align}
\frac{1}{\sqrt{1-x^2}} \cdot 2 \arcsin{x} \cdot e^{(\arcsin{x})^2} \\

\\
\frac{\cos x}{|\cos x|} 2 x \cdot e^{x^2}
\end{align}
$$

